Prove bnd lemmas
Only let app case
Prove result for subst
Prove for t_open_bound
Prove bnd preserved by t_make_wf

src/proofs/ElimLet/SubstitutionProofs.v
@@ -118,3 +118,675 @@ Proof.
   [apply t_make_wf_pres | | trans_case].
   intros. apply prove_errst_spec_ret. refl_case.
 Qed.
+
+(*Part 2: Spec*)
+Print t_subst_single1.
+Print t_subst1.
+Print term_traverse.
+Require Import TermFuncs Relations.
+
+Print eval_vsymbol.
+
+(*Get the list of new variable names.
+  NOTE: because eval_vsymbol is not compositional (it depends on more than 
+  just the encoded part), we can't express the names in terms of the core term
+  directly. But we can compute the list of names from the full term*)
+
+
+(*Get number of bound variables (only let)*)
+Fixpoint term_bnd (t: term_c) : nat :=
+  match t_node_of t with
+  | Tlet t1 (_, _, t2) => 1 + term_bnd t1 + term_bnd t2
+  | Tapp l tms => sum (map term_bnd tms)
+  | Tif t1 t2 t3 => term_bnd t1 + term_bnd t2 + term_bnd t3
+  | Tbinop _ t1 t2 => term_bnd t1 + term_bnd t2
+  | Tnot t1 => term_bnd t1
+  | _ => 0
+  end.
+
+Lemma term_bnd_rewrite t :
+  term_bnd t = match t_node_of t with
+  | Tlet t1 (_, _, t2) => 1 + term_bnd t1 + term_bnd t2
+  | Tapp l tms => sum (map term_bnd tms)
+  | Tif t1 t2 t3 => term_bnd t1 + term_bnd t2 + term_bnd t3
+  | Tbinop _ t1 t2 => term_bnd t1 + term_bnd t2
+  | Tnot t1 => term_bnd t1
+  | _ => 0
+  end.
+Proof. destruct t; auto. Qed.
+  
+
+(*Only bindings are let*)
+(*also only recursion is if, binop, not
+  no technical problems with app but makes proofs more annoying, could add later*)
+Fixpoint only_let (t: term_c) : bool :=
+  match t_node_of t with
+  | Tlet t1 (_, _, t2) => only_let t1 && only_let t2
+  | Tapp _ _ => false (*forallb (fun x => x) (map only_let tms)*)
+  | Tif t1 t2 t3 => only_let t1 && only_let t2 && only_let t3
+  | Tbinop _ t1 t2 => only_let t1 && only_let t2
+  | Tnot t1 => only_let t1
+  | Tcase _ _ => false
+  | Tquant _ _ => false
+  | Teps _ => false
+  | _ => true
+  end.
+
+Lemma only_let_rewrite t:
+  only_let t =
+   match t_node_of t with
+  | Tlet t1 (_, _, t2) => only_let t1 && only_let t2
+  | Tapp _ _ => false (*forallb (fun x => x) (map only_let tms)*)
+  | Tif t1 t2 t3 => only_let t1 && only_let t2 && only_let t3
+  | Tbinop _ t1 t2 => only_let t1 && only_let t2
+  | Tnot t1 => only_let t1
+  | Tcase _ _ => false
+  | Tquant _ _ => false
+  | Teps _ => false
+  | _ => true
+  end.
+Proof. destruct t; auto. Qed.
+
+(*And the core version*)
+Require Import Task.
+Print term.
+(*NOTE: if impl, could keep app, otherwise not*)
+Fixpoint only_let_tm (t: term) : bool :=
+  match t with
+  | Tlet t1 _ t2 => only_let_tm t1 && only_let_tm t2
+  | Tfun _ _ tms => forallb (fun x => x) (map only_let_tm tms)
+  | Tif f1 t1 t2 => only_let_fmla f1 && only_let_tm t1 && only_let_tm t2
+  | Tmatch _ _ _ => false
+  | Teps _ _ => false
+  | _ => true
+  end
+with only_let_fmla (f: formula) : bool :=
+  match f with
+  | Fpred _ _ tms => forallb (fun x => x) (map only_let_tm tms)
+  | Fquant _ _ _ => false
+  | Feq _ t1 t2 => only_let_tm t1 && only_let_tm t2
+  | Fbinop _ f1 f2 => only_let_fmla f1 && only_let_fmla f2
+  | Fnot f => only_let_fmla f
+  | Flet t1 _ f2 => only_let_tm t1 && only_let_fmla f2
+  | Fif f1 f2 f3 => only_let_fmla f1 && only_let_fmla f2 && only_let_fmla f3
+  | Fmatch _ _ _ => false
+  | _ => true
+  end.
+Require Import InversionLemmas.
+Set Bullet Behavior "Strict Subproofs".
+
+(*Now we want to prove: if [only_let t1] holds and t1 evaluates to e1, then 
+  [term_bnd t1] = length (term_bnd e1) (TODO: could prove only_let_tm holds but do separate)*)
+Lemma term_bnd_spec t1 (Ht1: only_let t1):
+  (forall e1 (Heval: eval_term t1 = Some e1), term_bnd t1 = length (tm_bnd e1)) /\
+  (forall e1 (Heval: eval_fmla t1 = Some e1), term_bnd t1 = length (fmla_bnd e1)).
+Proof.
+  induction t1 using term_ind_alt; split; intros e1 Heval; rewrite term_bnd_rewrite; try rewrite Heq;
+  try rewrite Ht; try (rewrite only_let_rewrite, Heq in Ht1; discriminate).
+  - rewrite (eval_var_tm Heq Heval). auto.
+  - exfalso; apply (eval_var_fmla Heq Heval).
+  - destruct (eval_const_tm Heq Heval) as [c1 [He1 Hc1]]; subst; auto.
+  - exfalso; apply (eval_const_fmla Heq Heval).
+  - (* rewrite only_let_rewrite, Heq in Ht1.
+    rewrite forallb_map in Ht1. destruct (eval_app_tm Heq Heval) as [f1 [tys' [tys1 [tms1 [He1 [Hf1 [Htys' [Htys1 Hts]]]]]]]].
+    subst. simpl. clear -H Hts Ht1. generalize dependent tms1.
+    induction ts as [| t1 tl IH]; simpl.
+    { intros [| t2 tl2]; try discriminate; auto. }
+    intros tms1 Hbind. inversion H as [| ? ? IH1 IH2]; subst; clear H.
+    simpl in Ht1. rewrite andb_true in Ht1; destruct Ht1 as [Honly1 Honly2].
+    apply option_bind_some in Hbind. destruct Hbind as [e2 [Ht1 Hbind]]. 
+    apply option_bind_some in Hbind. destruct Hbind as [l [Hfold Hl]]; inversion Hl; subst; clear Hl.
+    simpl. rewrite length_app. f_equal; auto. apply IH1; auto.
+  -  *)(*pred and eq*)
+    (*if*) destruct (eval_if_tm Heq Heval) as [e2 [e3 [e4 [He1 [He2 [He3 He4]]]]]]; subst.
+    simpl. rewrite !length_app. rewrite only_let_rewrite, Heq in Ht1. bool_hyps. rewrite !Nat.add_assoc.
+    f_equal; [f_equal|]; [apply IHt1_1 | apply IHt1_2 | apply IHt1_3]; auto. 
+  - destruct (eval_if_fmla Heq Heval) as [e2 [e3 [e4 [He1 [He2 [He3 He4]]]]]]; subst.
+    simpl. rewrite !length_app. rewrite only_let_rewrite, Heq in Ht1. bool_hyps. rewrite !Nat.add_assoc.
+    f_equal; [f_equal|]; [apply IHt1_1 | apply IHt1_2 | apply IHt1_3]; auto.
+  - (*let*) destruct (eval_let_tm Heq Heval) as [e2 [e3 [He1 [He2 He3]]]]; subst. simpl in *.
+    rewrite length_app. rewrite only_let_rewrite, Heq in Ht1. bool_hyps. f_equal. 
+    f_equal; [apply IHt1_1 | apply IHt1_2]; auto.
+  - destruct (eval_let_fmla Heq Heval) as [e2 [e3 [He1 [He2 He3]]]]; subst. simpl in *.
+    rewrite length_app. rewrite only_let_rewrite, Heq in Ht1. bool_hyps. f_equal. 
+    f_equal; [apply IHt1_1 | apply IHt1_2]; auto.
+  - (*binop*) exfalso. apply (eval_binop_tm Heq Heval).
+  - destruct (eval_binop_fmla Heq Heval) as [e2 [e3 [He1 [He2 He3]]]]. subst. simpl.
+    rewrite length_app. rewrite only_let_rewrite, Heq in Ht1. bool_hyps. 
+    f_equal; auto; [apply IHt1_1 | apply IHt1_2]; auto.
+  - (*not*) exfalso. apply (eval_not_tm Heq Heval).
+  - destruct (eval_not_fmla Heq Heval) as [e2 [He1 He2]]. subst. simpl.
+    rewrite only_let_rewrite, Heq in Ht1.
+    apply IHt1_1; auto.
+  - (*true*) exfalso. apply (eval_true_tm Ht Heval).
+  - rewrite (eval_true_fmla Ht Heval). reflexivity.
+  - (*false*) exfalso; apply (eval_false_tm Ht Heval).
+  - rewrite (eval_false_fmla Ht Heval); reflexivity.
+Qed.
+
+Lemma term_bnd_tm t1 (Ht1: only_let t1) e1 (Heval: eval_term t1 = Some e1): 
+  term_bnd t1 = length (tm_bnd e1).
+Proof. apply term_bnd_spec; auto. Qed.
+
+Lemma term_bnd_fmla t1 (Ht1: only_let t1) e1 (Heval: eval_fmla t1 = Some e1): 
+  term_bnd t1 = length (fmla_bnd e1).
+Proof. apply term_bnd_spec; auto. Qed.
+
+(*NOTE: we only care about let-bindings*)
+(*Let's do statefully for now*)
+Print ident.
+Definition ident_with (i: ident) (s: Z) :=
+  Build_ident (id_string i) (id_attrs i) (id_loc i) s.
+Print vsymbol.
+Definition vsym_with (v: TermDefs.vsymbol) (s: Z) := Build_vsymbol (ident_with (vs_name v) s) (vs_ty v).
+Print eval_vsymbol.
+Definition eval_vsym_str (v: TermDefs.vsymbol) : string :=
+  fst (eval_vsymbol v).
+Print Alpha.split_lens.
+
+Definition mapi {A B: Type} (f: nat -> A -> B) (l: list A) : list B :=
+  map (fun x => f (fst x) (snd x)) (combine (seq 0 (length l)) l).
+
+Local Open Scope Z_scope.
+(*For conversion, var has to go in middle*)
+(*Ignore Tquant, Teps, Tcase*)
+(*Won't do stateful, use bound info*)
+Fixpoint new_var_names (t: term_c) : Z -> list string :=
+  match t_node_of t with
+  | TermDefs.Tlet t1 (v, b, t2) => fun s =>
+    let s1 := s + Z.of_nat (term_bnd t1) in
+    let n1 := new_var_names t1 s in
+    let n2 := new_var_names t2 (Z.succ s1) in
+    eval_vsym_str (vsym_with v s1) :: n1 ++ n2
+    (* let (n2, s2) := new_var_names t2 (Z.succ s1) in
+    (eval_vsym_str (vsym_with v s1) :: n1 ++ n2, s2) *)
+  | Tapp l ts => fun s =>
+    (*A bit trickier, need to fold through, need to make so split_lens works*)
+    (*Idea: take the sum of term_bnd of the first i elements of ts*)
+    concat (mapi (fun i (f: Z -> list string) => f (Z.of_nat (sum (firstn i (map term_bnd ts))))) (map new_var_names ts))
+  | TermDefs.Tif t1 t2 t3 => fun s =>
+    let s1 := s + Z.of_nat (term_bnd t1) in
+    let s2 := s1 + Z.of_nat (term_bnd t2) in
+    let n1 := new_var_names t1 s in
+    let n2 := new_var_names t2 s1 in
+    let n3 := new_var_names t3 s2 in
+    n1 ++ n2 ++ n3
+  | Tbinop _ t1 t2 => fun s =>
+    let s1 := s + Z.of_nat (term_bnd t1) in
+    let n1 := new_var_names t1 s in
+    let n2 := new_var_names t2 s1 in
+    n1 ++ n2
+  | Tnot t => fun s => new_var_names t s
+  | _ => fun _ => nil
+  end.
+
+(* 
+
+fun s =>
+    (*Here, need to fold through - we write function in this way so we can map and apply value later*)
+    let l1 := map new_var_names ts in
+    fold_left (fun (acc: list string * Z) (x: Z -> list string * Z) =>
+      let (n, s) := acc in
+      let (n1, s1) := x s in
+      (n ++ n1, s1)) l1 (nil, s)
+  | Tif t1 t2 t3 => fun s =>
+    let (n1, s1) := new_var_names t1 s in
+    let (n2, s2) := new_var_names t2 s1 in
+    let (n3, s3) := new_var_names t3 s2 in
+    (n1 ++ n2 ++ n3, s3)
+  | Tbinop _ t1 t2 => fun s =>
+    let (n1, s1) := new_var_names t1 s in
+    let (n2, s2) := new_var_names t2 s1 in
+    (n1 ++ n2, s2)
+  | Tnot t1 => fun s => new_var_names t1 s
+  | _ => fun s => (nil, s)
+  end. *)
+
+(*old version*)
+(* Fixpoint new_var_names(t: term_c) : Z -> list string * Z :=
+  match t_node_of t with
+  | Tlet t1 (v, b, t2) => fun s =>
+    let (n1, s1) := new_var_names t1 s in
+    let (n2, s2) := new_var_names t2 (Z.succ s1) in
+    (eval_vsym_str (vsym_with v s1) :: n1 ++ n2, s2)
+  | Tapp l ts => fun s =>
+    (*Here, need to fold through - we write function in this way so we can map and apply value later*)
+    let l1 := map new_var_names ts in
+    fold_left (fun (acc: list string * Z) (x: Z -> list string * Z) =>
+      let (n, s) := acc in
+      let (n1, s1) := x s in
+      (n ++ n1, s1)) l1 (nil, s)
+  | Tif t1 t2 t3 => fun s =>
+    let (n1, s1) := new_var_names t1 s in
+    let (n2, s2) := new_var_names t2 s1 in
+    let (n3, s3) := new_var_names t3 s2 in
+    (n1 ++ n2 ++ n3, s3)
+  | Tbinop _ t1 t2 => fun s =>
+    let (n1, s1) := new_var_names t1 s in
+    let (n2, s2) := new_var_names t2 s1 in
+    (n1 ++ n2, s2)
+  | Tnot t1 => fun s => new_var_names t1 s
+  | _ => fun s => (nil, s)
+  end. *)
+
+Lemma new_var_names_rewrite t:
+  new_var_names t =
+   match t_node_of t with
+  | TermDefs.Tlet t1 (v, b, t2) => fun s =>
+    let s1 := s + Z.of_nat (term_bnd t1) in
+    let n1 := new_var_names t1 s in
+    let n2 := new_var_names t2 (Z.succ s1) in
+    eval_vsym_str (vsym_with v s1) :: n1 ++ n2
+    (* let (n2, s2) := new_var_names t2 (Z.succ s1) in
+    (eval_vsym_str (vsym_with v s1) :: n1 ++ n2, s2) *)
+  | Tapp l ts => fun s =>
+    (*A bit trickier, need to fold through, need to make so split_lens works*)
+    (*Idea: take the sum of term_bnd of the first i elements of ts*)
+    concat (mapi (fun i (f: Z -> list string) => f (Z.of_nat (sum (firstn i (map term_bnd ts))))) (map new_var_names ts))
+  | TermDefs.Tif t1 t2 t3 => fun s =>
+    let s1 := s + Z.of_nat (term_bnd t1) in
+    let s2 := s1 + Z.of_nat (term_bnd t2) in
+    let n1 := new_var_names t1 s in
+    let n2 := new_var_names t2 s1 in
+    let n3 := new_var_names t3 s2 in
+    n1 ++ n2 ++ n3
+  | Tbinop _ t1 t2 => fun s =>
+    let s1 := s + Z.of_nat (term_bnd t1) in
+    let n1 := new_var_names t1 s in
+    let n2 := new_var_names t2 s1 in
+    n1 ++ n2
+  | Tnot t => fun s => new_var_names t s
+  | _ => fun _ => nil
+  end.
+Proof. destruct t; auto. Qed.
+
+(* Lemma new_var_names_rewrite t:
+  new_var_names t = 
+  match t_node_of t with
+  | Tlet t1 (v, b, t2) => fun s =>
+    let (n1, s1) := new_var_names t1 s in
+    let (n2, s2) := new_var_names t2 (Z.succ s1) in
+    (eval_vsym_str (vsym_with v s1) :: n1 ++ n2, s2)
+  | Tapp l ts => fun s =>
+    (*Here, need to fold through - we write function in this way so we can map and apply value later*)
+    let l1 := map new_var_names ts in
+    fold_left (fun (acc: list string * Z) (x: Z -> list string * Z) =>
+      let (n, s) := acc in
+      let (n1, s1) := x s in
+      (n ++ n1, s1)) l1 (nil, s)
+  | Tif t1 t2 t3 => fun s =>
+    let (n1, s1) := new_var_names t1 s in
+    let (n2, s2) := new_var_names t2 s1 in
+    let (n3, s3) := new_var_names t3 s2 in
+    (n1 ++ n2 ++ n3, s3)
+  | Tbinop _ t1 t2 => fun s =>
+    let (n1, s1) := new_var_names t1 s in
+    let (n2, s2) := new_var_names t2 s1 in
+    (n1 ++ n2, s2)
+  | Tnot t1 => fun s => new_var_names t1 s
+  | _ => fun s => (nil, s)
+  end.
+Proof. destruct t; auto. Qed. *)
+
+(*And now the spec*)
+Print full_st.
+Require Import InversionLemmas.
+Require Import Alpha.
+Check alpha_t_aux.
+Require Import TermTactics.
+
+Set Bullet Behavior "Strict Subproofs".
+
+(*TODO: need resetriction on shape*)
+
+(*NOTE: we can't prove the general case for tm_traverse because the cases can do additional stateful operations*)
+Lemma errst_spec_pure_whole {St A} (P: Prop) (s: errState St A) (Q: St -> A -> St -> Prop):
+  (P -> errst_spec (fun _ => True) s Q) ->
+  errst_spec (fun _ => P) s Q.
+Proof.
+  intros Hp.
+  apply errst_spec_weaken_pre with (P1:=fun _ => True /\ P); [tauto|].
+  apply errst_spec_pure_pre; auto.
+Qed.
+
+(*TODO: move*)
+
+Lemma t_similar_only_let t s:
+  t_similar t s ->
+  only_let t = only_let s.
+Proof.
+  unfold t_similar. rewrite andb_true.
+  intros [Hoeq Hsim].
+  rewrite !only_let_rewrite.
+  destruct_term_node t; destruct_term_node s; try discriminate; auto; solve_similar.
+Qed.
+
+Lemma t_attr_copy_only_let t s:
+  only_let (t_attr_copy t s) = only_let s.
+Proof.
+  unfold t_attr_copy. destruct (_ && _) eqn : Hsim.
+  - apply t_similar_only_let. bool_hyps; auto.
+  - rewrite only_let_rewrite. simpl. rewrite only_let_rewrite. reflexivity.
+Qed.
+
+
+
+Lemma t_subst_unsafe_only_let (m: Mvs.t term_c) (Hm: forall x y, Mvs.find_opt x m = Some y -> only_let y)
+  t (Hlet: only_let t):
+  only_let (t_subst_unsafe_aux m t).
+Proof.
+  generalize dependent m.
+  induction t using term_ind_alt; rewrite only_let_rewrite in Hlet; try rewrite Heq in Hlet; try discriminate;
+  intros m Hm; rewrite TermTraverseAux.t_subst_unsafe_aux_rewrite; try rewrite Heq; try rewrite Ht;
+  try rewrite t_map_unsafe_rewrite; try rewrite Heq; try rewrite Ht; try rewrite t_attr_copy_only_let; auto; simpl.
+  - destruct_term_node t. unfold Mvs.find_def. inversion Heq; subst.
+    destruct (Mvs.find_opt v m) as [y|] eqn : Hfind; auto.
+    apply Hm in Hfind; auto.
+  - destruct_term_node t; auto.
+  - bool_hyps. bool_to_prop; split_all; [apply IHt1 | apply IHt2 | apply IHt3]; auto.
+  - rewrite andb_true in Hlet |- *. destruct Hlet as [Hlet1 Hlet2].
+    split; [apply IHt1; auto|]. destruct (Mvs.is_empty _ _) eqn : Hemp; auto.
+    apply IHt2; auto. eapply mvs_preserved; [| eauto]. apply binding_submap.
+  - bool_hyps. bool_to_prop. split; [apply IHt1 | apply IHt2]; auto.
+  - auto. 
+  - destruct_term_node t; auto.
+  - destruct_term_node t; auto.
+Qed.
+
+Lemma t_similar_bnd t s:
+  t_similar t s ->
+  term_bnd t = term_bnd s.
+Proof.
+  unfold t_similar. rewrite andb_true.
+  intros [Hoeq Hsim].
+  rewrite !term_bnd_rewrite.
+  destruct_term_node t; destruct_term_node s; try discriminate; auto; solve_similar.
+Qed.
+
+Lemma t_attr_copy_bnd t s:
+  term_bnd (t_attr_copy t s) = term_bnd s.
+Proof.
+  unfold t_attr_copy. destruct (_ && _) eqn : Hsim.
+  - apply t_similar_bnd. bool_hyps; auto.
+  - rewrite !term_bnd_rewrite. simpl. reflexivity.
+Qed.
+
+
+Lemma t_subst_unsafe_term_bnd (m: Mvs.t term_c) (Hm: forall x y, Mvs.find_opt x m = Some y -> term_bnd y = 0%nat)
+  t (Hlet: only_let t):
+  term_bnd (t_subst_unsafe_aux m t) = term_bnd t.
+Proof.
+  generalize dependent m. induction t using term_ind_alt; rewrite only_let_rewrite in Hlet; try rewrite Heq in Hlet; try discriminate;
+  intros m Hm; rewrite TermTraverseAux.t_subst_unsafe_aux_rewrite; try rewrite Heq; try rewrite Ht;
+  try rewrite t_map_unsafe_rewrite; try rewrite Heq; try rewrite Ht; try rewrite t_attr_copy_bnd; auto; simpl.
+  - destruct_term_node t. unfold Mvs.find_def. inversion Heq; subst. simpl.
+    destruct (Mvs.find_opt v m) as [y|] eqn : Hfind; auto.
+    apply Hm in Hfind; auto.
+  - destruct_term_node t4. inversion Heq; subst. bool_hyps. rewrite <- !Nat.add_assoc. f_equal; [| f_equal]; auto.
+  - destruct_term_node t3. inversion Heq; subst; simpl. bool_hyps. f_equal; auto. f_equal; auto.
+    destruct (Mvs.is_empty _ _) eqn : Hisemp; auto.
+    apply IHt2; auto. eapply mvs_preserved; [| eauto]. apply binding_submap.
+  - destruct_term_node t3. inversion Heq; subst. bool_hyps. f_equal; auto.
+  - destruct_term_node t2. inversion Heq; subst. auto.
+Qed. 
+
+Require Import StateHoareMonad.
+(*TODO: also prove only_let*)
+Lemma t_open_bound_bnd tb (Hlet: only_let (snd tb)):
+errst_spec (fun _ : full_st => True) (errst_tup1 (errst_lift1 (t_open_bound tb)))
+  (fun (_ : full_st) (tb1 : TermDefs.vsymbol * term_c) (_ : full_st) => only_let (snd tb1) /\ 
+    term_bnd (snd tb1) = term_bnd (snd tb)).
+Proof.
+  apply errst_spec_weaken with (P1:=fun _ => True /\ True) (Q1:=fun _ tb1 _ => 
+      (only_let (snd tb1) /\ term_bnd (snd tb1) = term_bnd (snd tb)) /\ True); auto.
+  { intros; tauto. }
+  apply errst_spec_tup1 with (P1:= fun _ => True) (P2:= fun _ tb1 _ => only_let (snd tb1) /\ term_bnd (snd tb1) = term_bnd (snd tb))
+    (Q1:=fun _ => True) (Q:=fun _ _ _ => True); auto.
+  apply errst_spec_st.
+  unfold t_open_bound. destruct tb as [[v1 b1] t1]; simpl.
+  eapply prove_st_spec_bnd_nondep with (Q2:=fun _ y _ => only_let (snd y) /\ term_bnd (snd y) = term_bnd t1); simpl; auto. 
+  { apply vs_rename_map. }
+  intros [m v]. simpl. apply prove_st_spec_ret. intros _ Hm. subst. simpl.
+  simpl in *.
+  split.
+  - unfold t_subst_unsafe. destruct (Mvs.is_empty _ _); auto.
+    apply t_subst_unsafe_only_let; auto.
+    intros x y. rewrite Mvs.add_spec. destruct (Vsym.Tg.equal x v1) eqn : Heq.
+    + inv Hsome. reflexivity.
+    + rewrite Mvs.empty_spec. discriminate.
+  - unfold t_subst_unsafe. destruct (Mvs.is_empty _ _); auto.
+    apply t_subst_unsafe_term_bnd; auto.
+    intros x y. rewrite Mvs.add_spec. destruct (Vsym.Tg.equal x v1) eqn : Heq.
+    + inv Hsome. reflexivity.
+    + rewrite Mvs.empty_spec. discriminate.
+Qed.
+
+(*First, prove bnd preserved by [t_wf]*)
+Lemma t_wf_bnd t (Hlet: only_let t):
+  errst_spec (fun (_: full_st) => True) (t_make_wf t) (fun _ t2 _ => term_bnd t2 = term_bnd t).
+Proof.
+  generalize dependent t. intros t. apply tm_traverse_ind with (P:=fun t x => forall (Hlet: only_let t),
+     errst_spec (fun (_: full_st) => True) x (fun _ t2 _ => term_bnd t2 = term_bnd t)); clear t.
+  - (*const*) intros t c Hn Hlet. apply prove_errst_spec_ret; auto.
+  - (*var*) intros t v Hn Hlet. apply prove_errst_spec_ret; auto.
+  - (*if*) intros t t1 t2 t3 Hn IH1 IH2 IH3 Hlet.
+    rewrite only_let_rewrite, Hn in Hlet. bool_hyps.
+    eapply prove_errst_spec_bnd_nondep'; [apply IH1 |]; auto. intros e1. simpl.
+    apply errst_spec_pure_whole. intros He1. 
+    eapply prove_errst_spec_bnd_nondep'; [apply IH2 |]; auto; intros e2. simpl.
+    apply errst_spec_pure_whole. intros He2.
+    eapply prove_errst_spec_bnd_nondep'; [apply IH3 |]; auto; intros e3. simpl.
+    apply errst_spec_pure_whole. intros He3.
+    (*Prove if*)
+    unfold tmap_if_default. apply errst_spec_err'. intros _ r Hif _.
+    unfold t_if in Hif. apply err_bnd_inr in Hif. destruct Hif as [u [_ Hbnd]].
+    apply err_bnd_inr in Hbnd. destruct Hbnd as [z [Hprop Hret]]. inversion Hret; subst.
+    simpl. unfold t_prop in Hprop. destruct (negb _); inversion Hprop; subst. 
+    destruct_term_node t. inversion Hn; subst. lia.
+  - (*let*) intros t t1 tb Hn IH1 IH2 Hlet. rewrite only_let_rewrite, Hn in Hlet.
+    destruct tb as [[v1 b1] t2]. bool_hyps.
+    eapply prove_errst_spec_bnd_nondep'; [apply IH1 |]; auto. intros e1. cbn beta. 
+    apply errst_spec_pure_whole. intros He1.
+    (*deal with [t_open_bound]*)
+    eapply prove_errst_spec_dep_bnd_nondep' with (Q1:=fun tb1 _ => term_bnd (snd tb1) = term_bnd t2).
+    + (*Prove result is [tm_bnd]*) eapply errst_spec_weaken_post. 2: apply t_open_bound_bnd; auto.
+      simpl. tauto.
+    + intros y s1 Hy. apply errst_spec_pure_whole. intros Htb2. 
+      eapply prove_errst_spec_bnd_nondep'; [eapply IH2; eauto |].
+      (*Now use fact that result is [only_let]*)
+      { (*Lost spec info so need to pose*)
+        pose proof (t_open_bound_bnd (v1, b1, t2) ltac:(auto)) as Hspec.
+        unfold errst_spec in Hspec. apply Hspec in Hy; auto. apply Hy.
+      }
+      simpl. intros e2. apply errst_spec_pure_whole. intros He2.
+      unfold tmap_let_default. apply errst_spec_err'. intros _ r Hr _.
+      unfold t_let_close, t_let, t_close_bound in Hr. apply err_bnd_inr in Hr.
+      destruct Hr as [u [_ Hret]]; inversion Hret; subst. simpl.
+      destruct_term_node t; inversion Hn; subst. lia.
+  - (*app - ruled out*)
+    intros t l ts Heq IH Hlet.
+    rewrite only_let_rewrite, Heq in Hlet. discriminate.
+  - (*case - ruled out*)
+    intros t t1 tbs Heq IH1 IH2 Hlet.
+    rewrite only_let_rewrite, Heq in Hlet. discriminate.
+  - (*eps - ruled out*)
+    intros t b Heq IH Hlet.
+    rewrite only_let_rewrite, Heq in Hlet. discriminate.
+  - (*quant - ruled out*)
+    intros t q tq Heq IH Hlet. 
+    rewrite only_let_rewrite, Heq in Hlet. discriminate.
+  - (*binop*) intros t b t1 t2 Hn IH1 IH2 Hlet.
+    rewrite only_let_rewrite, Hn in Hlet. bool_hyps.
+    eapply prove_errst_spec_bnd_nondep'; [apply IH1 |]; auto. intros e1. simpl.
+    apply errst_spec_pure_whole. intros He1. 
+    eapply prove_errst_spec_bnd_nondep'; [apply IH2 |]; auto; intros e2. simpl.
+    apply errst_spec_pure_whole. intros He2.
+    (*Prove op*)
+    unfold tmap_binop_default. apply errst_spec_err'. intros _ r Hb _.
+    unfold t_binary in Hb. apply err_bnd_inr in Hb. destruct Hb as [u [Hprop1 Hbnd]].
+    apply err_bnd_inr in Hbnd. destruct Hbnd as [z [Hprop2 Hret]]. inversion Hret; subst.
+    simpl. unfold t_prop in Hprop1, Hprop2. destruct (negb _); inversion Hprop1; subst.
+    destruct (negb _); inversion Hprop2; subst.
+    destruct_term_node t. inversion Hn; subst. lia.
+  - (*not*) intros t t1 Hn IH Hlet.
+    rewrite only_let_rewrite, Hn in Hlet. bool_hyps.
+    eapply prove_errst_spec_bnd_nondep'; [apply IH |]; auto. intros e1. simpl.
+    apply errst_spec_pure_whole. intros He1. 
+    (*Prove op*)
+    unfold tmap_binop_default. apply errst_spec_err'. intros _ r Hb _.
+    unfold t_not in Hb. apply err_bnd_inr in Hb. destruct Hb as [u [Hprop1 Hbnd]].
+    inversion Hbnd; subst. simpl. unfold t_prop in Hprop1. destruct (negb _); inversion Hprop1; subst.
+    destruct_term_node t. inversion Hn; subst. lia.
+  - (*true*) intros. apply prove_errst_spec_ret. auto.
+  - (*false*) intros. apply prove_errst_spec_ret. auto.
+Qed.
+
+
+Lemma t_wf_state t:
+  errst_spec (fun (_: full_st) => True) (t_make_wf t) (fun s1 _ s2 => fst s2 = Z.of_nat (term_bnd t) + fst s1).
+Proof. 
+  revert t.
+  apply tm_traverse_ind with (P:=fun t x =>
+    errst_spec (fun _ : full_st => True) x (fun s1 _ s2 => fst s2 = Z.of_nat (term_bnd t) + fst s1)).
+  - (*const*) intros t c Hn. apply prove_errst_spec_ret. destruct_term_node t. intros; lia.
+  - (*var*) intros t v Hn. apply prove_errst_spec_ret. destruct_term_node t. intros; lia.
+  - (*if*) intros t t1 t2 t3 Hn IH1 IH2 IH3.
+    eapply prove_errst_spec_bnd with (P2:= fun _ _ => True); [apply IH1 | | |].
+    (*TODO see*)
+    + intros e1. eapply prove_errst_spec_bnd with (P2:=fun _ _ => True)
+      (Q2:=fun _ s2 y s3 => ; [apply IH2 | | |].
+      * intros e2. eapply prove_errst_spec_bnd with (P2:=fun _ _ => True); [apply IH3 | | |].
+        -- intros e3. unfold tmap_if_default. apply errst_spec_err'.
+          intros i x Hif. 
+
+ Search errst_spec errst_lift2.
+
+
+ apply prove_errst_spec_ret.
+
+ apply IH3.
+
+(*NOTE: later prove length and NoDup for list*)
+(*NOTE: later, need to prove that under wf assumption, we have that no var in list appears*)
+Lemma t_wf_convert t1:
+  (forall e1 (Heval: eval_term t1 = Some e1),
+    errst_spec (fun (_: full_st) => True) (t_make_wf t1) (fun (s1: full_st) t2 _ =>
+      eval_term t2 = Some (alpha_t_aux e1 (new_var_names t1 (fst s1))))) /\
+  (forall e1 (Heval: eval_fmla t1 = Some e1),
+    errst_spec (fun (_: full_st) => True) (t_make_wf t1) (fun (s1: full_st) t2 _ =>
+      eval_fmla t2 = Some (alpha_f_aux e1 (new_var_names t1 (fst s1))))).
+Proof.
+  revert t1. apply tm_traverse_ind with (P:=fun t1 x =>
+      (forall e1 : term,
+   eval_term t1 = Some e1 ->
+   errst_spec (fun _ : CoqBigInt.t * TaskDefs.hashcons_full => True) x
+     (fun (s1 : full_st) (t2 : term_c) (_ : CoqBigInt.t * TaskDefs.hashcons_full) =>
+      eval_term t2 = Some (alpha_t_aux e1 (new_var_names t1 (fst s1))))) /\
+  (forall e1 : formula,
+   eval_fmla t1 = Some e1 ->
+   errst_spec (fun _ : CoqBigInt.t * TaskDefs.hashcons_full => True) x
+     (fun (s1 : full_st) (t2 : term_c) (_ : CoqBigInt.t * TaskDefs.hashcons_full) =>
+      eval_fmla t2 = Some (alpha_f_aux e1  (new_var_names t1 (fst s1)))))).
+  - (*const*) intros t1 c Heq. split; intros e1 Heval.
+    + apply prove_errst_spec_ret. intros i _.
+      rewrite new_var_names_rewrite, Heq. simpl.
+      destruct (eval_const_tm Heq Heval) as [c1 [He1 Hc1]]. subst.
+      simpl. auto.
+    + exfalso. apply (eval_const_fmla Heq Heval).
+  - (*var*) intros t1 v Heq; split; intros e1 Heval.
+    + apply prove_errst_spec_ret. intros i _.
+      rewrite new_var_names_rewrite, Heq. simpl.
+      rewrite (eval_var_tm Heq Heval) in Heval |- *. auto.
+    + exfalso. apply (eval_var_fmla Heq Heval).
+  - (*if*) intros t t1 t2 t3 Heq [_ IH1] [IH2 IH2'] [IH3 IH3']; split; intros e1 Heval.
+    + (*Tif*)
+      destruct (eval_if_tm Heq Heval) as [e2 [e3 [e4 [He1 [He2 [He3 He4]]]]]]; subst. simpl.
+      specialize (IH1 _ He2). 
+      (*TODO: need to prove that tm_make_wf increases state by exactly [term_wf t]*)
+      eapply prove_errst_spec_bnd with (Q1:=fun s1 t2 s2 =>
+        eval_fmla t2 = Some (alpha_f_aux e2 (new_var_names t1 (fst s1))) /\
+        fst s2 = Z.of_nat (term_bnd t1) + (fst s1))
+      (P2:=fun _ (_: full_st) => True) (*TODO see*)
+      (*TODO: not sure*)
+      (*s2 is state after 1st has been run before 2nd, s3 is state after 3rd*)
+      (Q2:= fun x s2 y s3 => 
+        let i := (fst s2) - Z.of_nat (term_bnd t1) in (*bad, but how else to recover orginal state?*)
+        eval_term y =
+        Some
+          (Tif (alpha_f_aux e2 (firstn (Datatypes.length (fmla_bnd e2)) (new_var_names t i)))
+             (alpha_t_aux e3
+                (firstn (Datatypes.length (tm_bnd e3))
+                   (skipn (Datatypes.length (fmla_bnd e2)) (new_var_names t i))))
+             (alpha_t_aux e4
+                (skipn (Datatypes.length (tm_bnd e3))
+                   (skipn (Datatypes.length (fmla_bnd e2)) (new_var_names t i)))))); auto.
+      3: { intros s1 s2 _ x y [Hevalx Hs12]. assert (Hfst: fst s1 = fst s2 - Z.of_nat (term_bnd t1)) by lia.
+        rewrite Hfst. auto. }
+      1: { (*prove first from IH*) apply errst_spec_split.
+
+
+        eval_term t3 = Some (alpha_t_aux e1 (new_var_names t2 (fst s1)))) 
+        
+      Search errst_spec errst_bind.
+
+
+
+      (*TODO: probably don't make stateful - just pass in number of bound vars
+        then will need to prove something about the values in the list: I guess:
+        all arise from evaluating a var with id between s and (s + length (tm_bnd t))
+        so we need a (at least count) of bound variables and to prove the equivalence
+        but we dont care about anything but let
+        1. define relation ruling out rest
+        2. define bnd count on term_c
+        3. redefine function above*)
+    
+
+
+ simpl. as [c1 [He1 Hc1]]. subst.
+      simpl. auto.
+
+
+      Search t_node_of TermDefs.Tconst.
+      
+
+
+
+
+ Search errst_spec errst_ret. 
+
+
+
+  Check tm_traverse_ind.
+  induction t1 using term_ind_alt.
+  - split; intros e1 Heval.
+    + (*Tvar*) rewrite t_make_wf_rewrite. 
+
+
+
+  errst_spec 
+
+  
+
+    fold_right (fun x acc => let (s1, n1) := x 
+    fold_right (fun 
+
+    let (n2, s2) := new_var_names 
+    (eval_vsym_str (vsym_with v s)) ++ 
+    
+
+
+Search errst_spec t_open_bound.
+(*NOTE: probably need to know that state is 1+ old old*)
+
+Print eval_vsymbol.
+
+
+(*Proofs about [t_make_wf]*)
+Search "a_convert".
+
+Print a_convert_t.
+
+
+
+
+
